code/experimental/gcm/Hacl.Standalone.GMAC.fst
@@ -22,273 +22,357 @@ open Hacl.Cast
 #set-options "--z3rlimit 20 --initial_fuel 0 --max_fuel 0 --initial_ifuel 0 --max_ifuel 0"
 
 (* GMAC state *)
-noeq type gmac_state = {ram:buffer H128.t; len:buffer U32.t}
-
-private let decode_pmsg (pmsg:H128.t) (len:U32.t{U32.v len <= 16}) : GTot word =
-  slice (big_bytes 16ul (H128.v pmsg)) 0 (U32.v len)
+noeq type gmac_state = {
+  r_acc : (b:buffer H128.t{length b =  2});
+  pmsg  : (b:buffer H8.t  {length b = 16});
+  len   : (b:buffer U32.t {length b =  1})}
 
 let live_st h (st:gmac_state) : Type0 =
-  live h st.ram /\ live h st.len /\ disjoint st.ram st.len
-
-let valid_pmsg (pmsg:H128.t) (len:U32.t) : Type0 =
-  U32.v len < 16 /\ pad (decode_pmsg pmsg len) = big_bytes 16ul (H128.v pmsg)
+  live h st.r_acc /\ live h st.pmsg /\ live h st.len /\
+  disjoint st.r_acc st.pmsg /\ disjoint st.r_acc st.len /\ disjoint st.pmsg st.len
 
 let valid_st h (st:gmac_state) : Type0 =
-  live_st h st /\ length st.ram = 3 /\ length st.len = 1 /\
-  valid_pmsg (get h st.ram 2) (get h st.len 0)
-  
+  live_st h st /\ U32.v (get h st.len 0) < 16
 
-(* Get information from state *)
-
-private let get_len h (st:gmac_state{valid_st h st}) : GTot U32.t = get h st.len 0
-
-private let get_r h (st:gmac_state{valid_st h st}) : GTot elem = sel_elem h (sub st.ram 0ul 1ul)
-private let get_acc h (st:gmac_state{valid_st h st}) : GTot elem = sel_elem h (sub st.ram 1ul 1ul)
-private let get_pmsg h (st:gmac_state{valid_st h st}) :
-  GTot (pmsg:bytes{Seq.length pmsg = U32.v (get h st.len 0)}) =
-  decode_pmsg (get h st.ram 2) (get h st.len 0)
+private let get_r h (st:gmac_state{live_st h st}) : GTot elem = sel_elem h (sub st.r_acc 0ul 1ul)
+private let get_acc h (st:gmac_state{live_st h st}) : GTot elem = sel_elem h (sub st.r_acc 1ul 1ul)
+private let get_pmsg h (st:gmac_state{valid_st h st}) : GTot bytes =
+  reveal_sbytes (slice (as_seq h st.pmsg) 0 (U32.v (get h st.len 0)))
 
 private val as_pure_st: h:HyperStack.mem -> st:gmac_state{valid_st h st} -> GTot (pst:gmac_state_)
 let as_pure_st h st = MkState (get_r h st) (get_acc h st) (get_pmsg h st)
 
 
+(* Assistant functions *)
+
+#reset-options "--z3rlimit 50 --initial_fuel 1 --max_fuel 1 --initial_ifuel 0 --max_ifuel 0"
+
+private abstract val gmac_pmsg_concat: st:gmac_state ->
+  msg:buffer H8.t{disjoint st.r_acc msg /\ disjoint st.pmsg msg /\ disjoint st.len msg} ->
+  l:U32.t{length msg = U32.v l} ->
+  Stack unit
+  (requires (fun h -> valid_st h st /\ live h msg /\ U32.v (get h st.len 0) + U32.v l <= 16))
+  (ensures (fun h0 _ h1 -> valid_st h0 st /\ live h0 msg /\ live_st h1 st /\ live h1 msg /\
+    modifies_2 st.pmsg st.len h0 h1 /\
+    get_r h0 st = get_r h1 st /\ get_acc h0 st = get_acc h1 st /\
+    U32.v (get h1 st.len 0) = U32.v (get h0 st.len 0) + U32.v l /\
+    U32.v (get h1 st.len 0) <= 16 /\
+    reveal_sbytes (slice (as_seq h1 st.pmsg) 0 (U32.v (get h1 st.len 0))) = get_pmsg h0 st @| reveal_sbytes (as_seq h0 msg)))
+let gmac_pmsg_concat st msg l =
+  let h0 = ST.get() in
+  let pl = st.len.(0ul) in
+  blit msg 0ul st.pmsg pl l;
+  st.len.(0ul) <- U32.(pl +^ l);
+  let h1 = ST.get() in
+  assert(disjoint st.pmsg (sub st.r_acc 0ul 1ul));
+  assert(disjoint st.pmsg (sub st.r_acc 1ul 1ul));
+  let pmsg_1 = reveal_sbytes (slice (as_seq h1 st.pmsg) 0 (U32.v (get h1 st.len 0))) in
+  lemma_eq_intro (slice (as_seq h1 st.pmsg) 0 (U32.v pl)) (slice (as_seq h0 st.pmsg) 0 (U32.v pl));
+  lemma_eq_intro (slice pmsg_1 0 (U32.v pl)) (get_pmsg h0 st);
+  lemma_eq_intro (slice (reveal_sbytes (as_seq h1 st.pmsg)) (U32.v pl) (U32.v pl + U32.v l)) (reveal_sbytes (slice (as_seq h1 st.pmsg) (U32.v pl) (U32.v pl + U32.v l)));
+  lemma_eq_intro (slice (as_seq h1 st.pmsg) (U32.v pl) (U32.v pl + U32.v l)) (as_seq h0 msg);
+  lemma_eq_intro pmsg_1 (get_pmsg h0 st @| reveal_sbytes (as_seq h0 msg))
+
 #reset-options "--z3rlimit 50 --initial_fuel 0 --max_fuel 0 --initial_ifuel 0 --max_ifuel 0"
 
-(* Useful lemmas *)
+private abstract val gmac_pmsg_padding: st:gmac_state ->
+  Stack unit
+  (requires (fun h -> valid_st h st /\ U32.v (get h st.len 0) > 0))
+  (ensures (fun h0 _ h1 -> valid_st h0 st /\ live_st h1 st /\
+    modifies_1 st.pmsg h0 h1 /\
+    get_r h0 st = get_r h1 st /\ get_acc h0 st = get_acc h1 st /\
+    reveal_sbytes (as_seq h1 st.pmsg) = get_pmsg h0 st @| Seq.create (16 - U32.v (get h0 st.len 0)) 0uy))
+let gmac_pmsg_padding st =
+  let h0 = ST.get() in
+  let pl = st.len.(0ul) in
+  let pmsg = sub st.pmsg 0ul pl in
+  let rest = sub st.pmsg pl U32.(16ul -^ pl) in
+  fill rest (uint8_to_sint8 0uy) U32.(16ul -^ pl);
+  let h' = ST.get() in
+  assert(disjoint pmsg rest);
+  lemma_reveal_modifies_1 rest h0 h';
+  let h1 = ST.get() in
+  lemma_eq_intro (reveal_sbytes (as_seq h1 st.pmsg)) (reveal_sbytes (slice (as_seq h1 st.pmsg) 0 (U32.v pl)) @| reveal_sbytes (slice (as_seq h1 st.pmsg) (U32.v pl) 16));
+  lemma_eq_intro (reveal_sbytes (slice (as_seq h1 st.pmsg) 0 (U32.v pl))) (get_pmsg h0 st);
+  lemma_eq_intro (slice (as_seq h1 st.pmsg) (U32.v pl) 16) (slice (as_seq h1 rest) 0 (16 - U32.v pl));
+  lemma_eq_intro (slice (as_seq h1 rest) 0 (16 - U32.v pl)) (Seq.create (16 - U32.v pl) (uint8_to_sint8 0uy));
+  lemma_eq_intro (reveal_sbytes (Seq.create (16 - U32.v pl) (uint8_to_sint8 0uy))) (Seq.create (16 - U32.v (get h0 st.len 0)) 0uy)
 
-private let valid_pmsg_ (pmsg:H128.t) (len:U32.t) : Type0 =
-  U32.v len < 16 /\ H128.v pmsg % (pow2 (8 * (16 - U32.v len))) = 0
-
-private val zero_div_mod: n:pos -> Lemma (0 / n = 0 /\ 0 % n = 0)
-let zero_div_mod n = Math.Lemmas.multiple_division_lemma 0 n; Math.Lemmas.multiple_modulo_lemma 0 n
-
-private val lemma_is_valid_pmsg_: pmsg:H128.t -> len:U32.t{valid_pmsg_ pmsg len} -> i:nat{i < 16 - U32.v len} ->
-  Lemma (requires True)
-  (ensures (Seq.index (slice (big_bytes 16ul (H128.v pmsg)) (U32.v len) 16) i = 0uy))
-  [SMTPat (Seq.index (slice (big_bytes 16ul (H128.v pmsg)) (U32.v len) 16) i)]
-let lemma_is_valid_pmsg_ pmsg len i =
-  lemma_index_big_bytes 16ul (H128.v pmsg) (U32.v len + i);
-  Math.Lemmas.pow2_modulo_division_lemma_1 (H128.v pmsg) (8 * (16 - U32.v len - i - 1)) (8 * (16 - U32.v len - i));
-  Math.Lemmas.pow2_modulo_modulo_lemma_1 (H128.v pmsg) (8 * (16 - U32.v len - i)) (8 * (16 - U32.v len));
-  zero_div_mod (pow2 (8 * (16 - U32.v len - i)));
-  zero_div_mod (pow2 (8 * (16 - U32.v len - i - 1)))
+#reset-options "--z3rlimit 50 --initial_fuel 1 --max_fuel 1 --initial_ifuel 0 --max_ifuel 0"
   
-private val lemma_is_valid_pmsg: pmsg:H128.t -> len:U32.t -> Lemma
-  (requires (valid_pmsg_ pmsg len))
-  (ensures (valid_pmsg pmsg len))
-  [SMTPat (valid_pmsg pmsg len)]
-let lemma_is_valid_pmsg pmsg len =
-  lemma_eq_intro (Seq.create (16 - U32.v len) 0uy) (slice (big_bytes 16ul (H128.v pmsg)) (U32.v len) 16);
-  lemma_eq_intro (pad (decode_pmsg pmsg len)) (big_bytes 16ul (H128.v pmsg))
-  
+private abstract val gmac_update_short: st:gmac_state ->
+  msg:buffer H8.t{disjoint st.r_acc msg /\ disjoint st.pmsg msg /\ disjoint st.len msg} ->
+  l:U32.t{length msg = U32.v l} ->
+  Stack unit
+  (requires (fun h -> valid_st h st /\ live h msg /\ U32.v (get h st.len 0) + U32.v l < 16))
+  (ensures (fun h0 _ h1 -> valid_st h0 st /\ live h0 msg /\ valid_st h1 st /\ live h1 msg /\
+    modifies_2 st.pmsg st.len h0 h1 /\ 
+    as_pure_st h1 st = gmac_update_spec (as_pure_st h0 st) (as_seq h0 msg)))
+let gmac_update_short st msg l =
+  let h0 = ST.get() in
+  if U32.v l = 0 then lemma_eq_intro (get_pmsg h0 st) (get_pmsg h0 st @| reveal_sbytes (as_seq h0 msg))
+  else gmac_pmsg_concat st msg l
+
+#reset-options "--z3rlimit 100 --initial_fuel 0 --max_fuel 0 --initial_ifuel 0 --max_ifuel 0"
+
+(* NOTE: The spec is very lax. Make sure the pmsg is full before calling and set st.len as 0ul right after. *)
+private abstract val gmac_full_pmsg_absorb: st:gmac_state -> Stack unit
+  (requires (fun h -> live_st h st))
+  (ensures (fun h0 _ h1 -> live_st h0 st /\ live_st h1 st /\
+    modifies_1 st.r_acc h0 h1 /\ get_r h0 st = get_r h1 st /\
+    get_acc h1 st = (get_acc h0 st +@ encode (reveal_sbytes (as_seq h0 st.pmsg))) *@ get_r h0 st))
+let gmac_full_pmsg_absorb st =
+  let h0 = ST.get() in
+  let r = sub st.r_acc 0ul 1ul in
+  let acc = sub st.r_acc 1ul 1ul in
+  let bv = encodeB st.pmsg in
+  acc.(0ul) <- H128.(acc.(0ul) ^^ bv);
+  gf128_mul acc r;
+  let h1 = ST.get() in
+  assert(disjoint acc r);
+  assert(disjoint acc st.len);
+  lemma_reveal_modifies_1 acc h0 h1
+
+private abstract val gmac_update_short_3: st:gmac_state ->
+  msg:buffer H8.t{disjoint st.r_acc msg /\ disjoint st.pmsg msg /\ disjoint st.len msg} ->
+  l:U32.t{length msg = U32.v l} ->
+  Stack unit
+  (requires (fun h -> valid_st h st /\ live h msg /\ U32.v (get h st.len 0) + U32.v l < 16))
+  (ensures (fun h0 _ h1 -> valid_st h0 st /\ live h0 msg /\ valid_st h1 st /\ live h1 msg /\
+    modifies_3 st.r_acc st.pmsg st.len h0 h1 /\ 
+    as_pure_st h1 st = gmac_update_spec (as_pure_st h0 st) (as_seq h0 msg)))
+let gmac_update_short_3 st msg l =
+  let h0 = ST.get() in
+  gmac_update_short st msg l;
+  let h1 = ST.get() in
+  lemma_reveal_modifies_2 st.pmsg st.len h0 h1;
+  lemma_intro_modifies_3 st.r_acc st.pmsg st.len h0 h1
+
+#reset-options "--z3rlimit 200 --initial_fuel 0 --max_fuel 0 --initial_ifuel 0 --max_ifuel 0"
+
+private abstract val gmac_update_exact_block: st:gmac_state ->
+  msg:buffer H8.t{disjoint st.r_acc msg /\ disjoint st.pmsg msg /\ disjoint st.len msg} ->
+  l:U32.t{length msg = U32.v l} ->
+  Stack unit
+  (requires (fun h -> valid_st h st /\ live h msg /\ U32.v (get h st.len 0) + U32.v l = 16))
+  (ensures (fun h0 _ h1 -> valid_st h0 st /\ live h0 msg /\ valid_st h1 st /\ live h1 msg /\
+    modifies_3 st.r_acc st.pmsg st.len h0 h1 /\ 
+    as_pure_st h1 st = gmac_update_spec (as_pure_st h0 st) (as_seq h0 msg)))
+let gmac_update_exact_block st msg l =
+  let h0 = ST.get() in
+  lemma_gmac_update_exact_block (as_pure_st h0 st) (as_seq h0 msg);
+  gmac_pmsg_concat st msg l;
+  let h' = ST.get() in
+  lemma_eq_intro (as_seq h' st.pmsg) (slice (as_seq h' st.pmsg) 0 (U32.v (get h' st.len 0)));
+  lemma_sub_spec st.r_acc 0ul 1ul h0;
+  lemma_sub_spec st.r_acc 0ul 1ul h';
+  lemma_sub_spec st.r_acc 1ul 1ul h0;
+  lemma_sub_spec st.r_acc 1ul 1ul h';
+  lemma_reveal_modifies_2 st.pmsg st.len h0 h';
+  gmac_full_pmsg_absorb st;
+  st.len.(0ul) <- 0ul;
+  let h1 = ST.get() in
+  lemma_eq_intro (get_pmsg h1 st) createEmpty;
+  lemma_reveal_modifies_2 st.r_acc st.len h' h1;
+  lemma_intro_modifies_3 st.r_acc st.pmsg st.len h0 h1
+
+#reset-options "--z3rlimit 200 --initial_fuel 1 --max_fuel 1 --initial_ifuel 0 --max_ifuel 0"
+
+abstract val gmac_update_0: st:gmac_state ->
+  msg:buffer H8.t{disjoint st.r_acc msg /\ disjoint st.pmsg msg /\ disjoint st.len msg} ->
+  l:U32.t{length msg = U32.v l} ->
+  Stack unit
+  (requires (fun h -> valid_st h st /\ live h msg /\ get_pmsg h st = createEmpty))
+  (ensures (fun h0 _ h1 -> valid_st h0 st /\ live h0 msg /\ valid_st h1 st /\ live h1 msg /\
+    modifies_3 st.r_acc st.pmsg st.len h0 h1 /\ 
+    as_pure_st h1 st = gmac_update_spec (as_pure_st h0 st) (as_seq h0 msg)))
+  (decreases (length msg))
+let rec gmac_update_0 st msg l =
+  let h0 = ST.get() in
+  if U32.v l < 16 then gmac_update_short_3 st msg l
+  else begin
+    let block = sub msg 0ul 16ul in
+    lemma_eq_intro (reveal_sbytes (as_seq h0 block)) (get_pmsg h0 st @| reveal_sbytes (slice (as_seq h0 msg) 0 16));
+    let nmsg = sub msg 16ul U32.(l -^ 16ul) in
+    let r = sub st.r_acc 0ul 1ul in
+    let acc = sub st.r_acc 1ul 1ul in
+    let bv = encodeB block in
+    acc.(0ul) <- H128.(acc.(0ul) ^^ bv);
+    gf128_mul acc r;
+    let h' = ST.get() in
+    lemma_reveal_modifies_1 acc h0 h';
+    lemma_intro_modifies_3 st.r_acc st.pmsg st.len h0 h';
+    gmac_update_0 st nmsg U32.(l -^ 16ul);
+    let h1 = ST.get() in
+    lemma_modifies_3_trans st.r_acc st.pmsg st.len h0 h' h1
+  end
+
+#reset-options "--z3rlimit 100 --initial_fuel 0 --max_fuel 0 --initial_ifuel 0 --max_ifuel 0"
+
+private abstract val gmac_last_nonempty: st:gmac_state -> Stack unit
+  (requires (fun h -> valid_st h st /\ U32.v (get h st.len 0) > 0))
+  (ensures (fun h0 _ h1 -> valid_st h0 st /\ valid_st h1 st /\
+    modifies_2 st.r_acc st.pmsg h0 h1 /\
+    get_acc h1 st = (get_acc h0 st +@ encode (get_pmsg h0 st)) *@ get_r h0 st))
+let gmac_last_nonempty st =
+  let h0 = ST.get() in
+  gmac_pmsg_padding st;
+  let h' = ST.get() in
+  gmac_full_pmsg_absorb st;
+  let h1 = ST.get() in
+  lemma_eq_intro (pad (get_pmsg h0 st)) (pad (get_pmsg h0 st @| Seq.create (16 - U32.v (get h0 st.len 0)) 0uy))
+
+#reset-options "--z3rlimit 50 --initial_fuel 1 --max_fuel 1 --initial_ifuel 0 --max_ifuel 0"
+
+private abstract val gmac_last_: st:gmac_state -> Stack unit
+  (requires (fun h -> valid_st h st))
+  (ensures (fun h0 _ h1 -> valid_st h0 st /\ valid_st h1 st /\
+    modifies_2 st.r_acc st.pmsg h0 h1 /\
+    get_acc h1 st = gmac_last_spec (as_pure_st h0 st)))
+let gmac_last_ st =
+  let pl = st.len.(0ul) in
+  if U32.v pl = 0 then () else gmac_last_nonempty st
+
 
 (* Main functions *)
 
-#reset-options "--z3rlimit 80 --initial_fuel 0 --max_fuel 0 --initial_ifuel 0 --max_ifuel 0"
+#reset-options "--z3rlimit 100 --initial_fuel 0 --max_fuel 0 --initial_ifuel 0 --max_ifuel 0"
 
-val gmac_alloc: unit -> StackInline gmac_state
+abstract val gmac_alloc: unit -> StackInline gmac_state
   (requires (fun _ -> True))
-  (ensures (fun h0 st h1 -> ~(contains h0 st.ram) /\ ~(contains h0 st.len) /\
-    frameOf st.ram == h0.tip /\ frameOf st.len == h0.tip /\
-    modifies_0 h0 h1 /\ valid_st h1 st))
+  (ensures (fun h0 st h1 -> ~(contains h0 st.r_acc) /\ ~(contains h0 st.pmsg) /\ ~(contains h0 st.len) /\
+    frameOf st.r_acc == h0.tip /\ frameOf st.pmsg == h0.tip /\ frameOf st.len == h0.tip /\
+    modifies_0 h0 h1 /\ valid_st h1 st /\
+    as_pure_st h1 st = gmac_alloc_spec))
 let gmac_alloc () =
   let h0 = ST.get() in
-  let ram = create zero_128 3ul in
+  let r_acc = create zero_128 2ul in
+  fzero_lemma zero_128;
   let h1 = ST.get() in
   lemma_reveal_modifies_0 h0 h1;
+  let pmsg = create (uint8_to_sint8 0uy) 16ul in
+  let h2 = ST.get() in
+  lemma_reveal_modifies_0 h1 h2;
   let len = create 0ul 1ul in
-  {ram = ram; len = len}
+  let h3 = ST.get() in
+  let st = {r_acc = r_acc; pmsg = pmsg; len = len} in
+  lemma_eq_intro (get_pmsg h3 st) createEmpty;
+  st
 
-val gmac_init: st:gmac_state -> r:keyB{disjoint st.ram r /\ disjoint st.len r} -> Stack unit
+abstract val gmac_init: st:gmac_state ->
+  r:keyB{disjoint st.r_acc r /\ disjoint st.pmsg r /\ disjoint st.len r} ->
+  Stack unit
   (requires (fun h -> valid_st h st /\ live h r))
   (ensures (fun h0 _ h1 -> valid_st h0 st /\ live h0 r /\ valid_st h1 st /\ live h1 r /\
-    modifies_2 st.ram st.len h0 h1 /\
+    modifies_2 st.r_acc st.len h0 h1 /\
     as_pure_st h1 st = gmac_init_spec (as_seq h0 r)))
 let gmac_init st r =
   let h0 = ST.get() in
   let rv = encodeB r in
-  st.ram.(0ul) <- rv;
-  st.ram.(1ul) <- zero_128;
-  st.ram.(2ul) <- zero_128;
+  st.r_acc.(0ul) <- rv;
+  st.r_acc.(1ul) <- zero_128;
   st.len.(0ul) <- 0ul;
   let h1 = ST.get() in
-  zero_div_mod (pow2 (8 * 16));
-  Seq.lemma_eq_intro (get_r h1 st) (encode (reveal_sbytes (as_seq h0 r)));
+  lemma_eq_intro (get_r h1 st) (encode (reveal_sbytes (as_seq h0 r)));
   fzero_lemma zero_128;
-  Seq.lemma_eq_intro (get_acc h1 st) zero;
-  Seq.lemma_eq_intro (get_pmsg h1 st) (Seq.createEmpty)
+  lemma_eq_intro (get_acc h1 st) zero;
+  lemma_eq_intro (get_pmsg h1 st) createEmpty
 
-private val update_pmsg: pmsg:H128.t -> len_1:U32.t{valid_pmsg_ pmsg len_1} ->
-  nmsg:wordB -> len_2:U32.t{length nmsg = U32.v len_2 /\ U32.(v (len_1 +^ len_2)) <= 16} -> StackInline H128.t
-  (requires (fun h -> live h nmsg))
-  (ensures (fun h0 r h1 -> live h0 nmsg /\ modifies_0 h0 h1 /\ valid_pmsg_ r U32.(len_1 +^ len_2) /\
-    decode_pmsg r U32.(len_1 +^ len_2) = decode_pmsg pmsg len_1 @| reveal_sbytes (as_seq h0 nmsg)))
-let update_pmsg pmsg len_1 nmsg len_2 =
-  let h0 = ST.get() in
-  push_frame();
-  let nmsg_16 = create (uint8_to_sint8 0uy) 16ul in
-  blit nmsg 0ul nmsg_16 len_1 len_2;
-  let h' = ST.get() in
-  let pmsg_ = encodeB nmsg_16 in
-  pop_frame();
-  let h1 = ST.get() in
-  lemma_eq_intro (slice ( (as_seq h' nmsg_16)) (U32.v len_1) (U32.v len_1 + U32.v len_2)) ( (as_seq h0 nmsg));
-  admit()
-  (*
-  admit();
-  lemma_eq_intro (sel_word h' nmsg_16) (pad (sel_word h' nmsg_16));
-  FStar.UInt.to_vec_lemma_2 (big_endian (sel_word h' nmsg_16)) (H128.v pmsg_);
-  assert(big_endian (sel_word h' nmsg_16) = H128.v pmsg_);
-  lemma_eq_intro (Seq.create (U32.v len_1) 0uy) (slice (sel_word h' nmsg_16) 0 (U32.v len_1));
-  admit();
-  lemma_eq_intro (Seq.create (U32.v len_1) 0uy @| slice (sel_word h' nmsg_16) (U32.v len_1) 16)
-    (sel_word h' nmsg_16);
-  admit();
-  *)
-  assume(H128.v pmsg + H128.v pmsg_ < pow2 128);
-  assume(valid_pmsg_ H128.(pmsg +^ pmsg_) U32.(len_1 +^ len_2));
-  assume(slice (decode_pmsg H128.(pmsg +^ pmsg_) U32.(len_1 +^ len_2)) 0 (U32.v len_1) = decode_pmsg pmsg len_1);
-  assume(slice (decode_pmsg H128.(pmsg +^ pmsg_) U32.(len_1 +^ len_2)) (U32.v len_1) (U32.v len_1 + U32.v len_2) = reveal_sbytes (as_seq h0 nmsg));
-  lemma_eq_intro (decode_pmsg H128.(pmsg +^ pmsg_) U32.(len_1 +^ len_2)) (decode_pmsg pmsg len_1 @| reveal_sbytes (as_seq h0 nmsg));
-  H128.(pmsg +^ pmsg_)
-  
-
-val gmac_update: st:gmac_state -> msg:buffer H8.t{disjoint st.ram msg /\ disjoint st.len msg} -> Stack unit
+abstract val gmac_update: st:gmac_state ->
+  msg:buffer H8.t{disjoint st.r_acc msg /\ disjoint st.pmsg msg /\ disjoint st.len msg} ->
+  l:U32.t{length msg = U32.v l} ->
+  Stack unit
   (requires (fun h -> valid_st h st /\ live h msg))
   (ensures (fun h0 _ h1 -> valid_st h0 st /\ live h0 msg /\ valid_st h1 st /\ live h1 msg /\
-    modifies_2 st.ram st.len h0 h1 /\
-    as_pure_st h1 st = gmac_update_spec (as_pure_st h0 st) (sel_word h0 msg)))
-let gmac_update st msg = admit()
+    modifies_3 st.r_acc st.pmsg st.len h0 h1 /\
+    as_pure_st h1 st = gmac_update_spec (as_pure_st h0 st) (as_seq h0 msg)))
+let gmac_update st msg l =
+  let h0 = ST.get() in
+  let pl = st.len.(0ul) in
+  if U32.v pl + U32.v l < 16 then gmac_update_short_3 st msg l
+  else begin
+    let msg_1 = sub msg 0ul U32.(16ul -^ pl) in
+    let msg_2 = sub msg U32.(16ul -^ pl) U32.(l -^ (16ul -^ pl)) in
+    gmac_update_exact_block st msg_1 U32.(16ul -^ pl);
+    let h' = ST.get() in
+    lemma_reveal_modifies_3 st.r_acc st.pmsg st.len h0 h';
+    lemma_sub_spec msg U32.(16ul -^ pl) U32.(l -^ (16ul -^ pl)) h0;
+    lemma_sub_spec msg U32.(16ul -^ pl) U32.(l -^ (16ul -^ pl)) h';
+    lemma_eq_intro (get_pmsg h' st) createEmpty;
+    gmac_update_0 st msg_2 U32.(l -^ (16ul -^ pl));
+    let h1 = ST.get() in
+    lemma_gmac_update_ (as_pure_st h0 st) (as_seq h0 msg_1) (as_seq h' msg_2);
+    lemma_eq_intro (as_seq h0 msg) (as_seq h0 msg_1 @| as_seq h0 msg_2);
+    lemma_modifies_3_trans st.r_acc st.pmsg st.len h0 h' h1
+  end
 
-
-(*
-inline_for_extraction private
-val gmac_set_r: st:gmac_state -> r:wordB_16{disjoint st.r_acc r /\ disjoint st.s_pmsg_len r} -> Stack unit
-  (requires (fun h -> valid_st h st /\ live h r))
-  (ensures (fun h0 _ h1 -> valid_st h0 st /\ live h0 r /\ valid_st h1 st /\ live h1 r /\
+abstract val gmac_update_block: st:gmac_state ->
+  msg:tagB{disjoint st.r_acc msg /\ disjoint st.pmsg msg /\ disjoint st.len msg} ->
+  Stack unit
+  (requires (fun h -> valid_st h st /\ live h msg /\ get_pmsg h st = createEmpty))
+  (ensures (fun h0 _ h1 -> valid_st h0 st /\ live h0 msg /\ valid_st h1 st /\ live h1 msg /\
     modifies_1 st.r_acc h0 h1 /\
-    get_r h1 st = encode (as_seq h0 r) /\ get_s h1 st = get_s h0 st /\
-    get_acc h1 st = get_acc h0 st /\ get_pmsg h1 st = get_pmsg h0 st))
-let gmac_set_r st r =
+    as_pure_st h1 st = gmac_update_spec (as_pure_st h0 st) (as_seq h0 msg)))
+let gmac_update_block st msg =
   let h0 = ST.get() in
-  let st_r = sub st.r_acc 0ul 1ul in
-  let rv = load128_be r in
-  st_r.(0ul) <- rv;
+  lemma_eq_intro (get_pmsg h0 st @| reveal_sbytes (as_seq h0 msg)) (reveal_sbytes (as_seq h0 msg));
+  let r = sub st.r_acc 0ul 1ul in
+  let acc = sub st.r_acc 1ul 1ul in
+  let bv = encodeB msg in
+  acc.(0ul) <- H128.(acc.(0ul) ^^ bv);
+  gf128_mul acc r;
   let h1 = ST.get() in
-  (* get_r h1 st = encode (as_seq h0 r) *)
-  Seq.lemma_eq_intro (get_r h1 st) (encode (as_seq h0 r));
-  (* get_acc h1 st = get_acc h0 st *)
-  let st_acc = sub st.r_acc 1ul 1ul in
-  assert(disjoint st_r st_acc);
-  lemma_reveal_modifies_1 st_r h0 h1;
-  (* get_s h1 st = get_s h0 st *)
-  lemma_sub_spec st.s_pmsg_len 0ul 16ul h0;
-  lemma_sub_spec st.s_pmsg_len 0ul 16ul h1;
-  (* get_pmsg h1 st = get_pmsg h0 st *)
-  lemma_sub_spec st.s_pmsg_len 16ul (h8_to_u32 (get h0 st.s_pmsg_len 32)) h0;
-  lemma_sub_spec st.s_pmsg_len 16ul (h8_to_u32 (get h1 st.s_pmsg_len 32)) h1
+  assert(disjoint acc r);
+  lemma_reveal_modifies_1 acc h0 h1;
+  lemma_gmac_update_exact_block (as_pure_st h0 st) (as_seq h0 msg)
 
-inline_for_extraction private
-val gmac_set_s: st:gmac_state -> s:tagB{disjoint st.r_acc s /\ disjoint st.s_pmsg_len s} -> Stack unit
-  (requires (fun h -> valid_st h st /\ live h s))
-  (ensures (fun h0 _ h1 -> valid_st h0 st /\ live h0 s /\ valid_st h1 st /\ live h1 s /\
-    modifies_1 st.s_pmsg_len h0 h1 /\
-    get_r h1 st = get_r h0 st /\ get_s h1 st = as_seq h0 s /\
-    get_acc h1 st = get_acc h0 st /\ get_pmsg h1 st = get_pmsg h0 st))
-let gmac_set_s st s =
+abstract val gmac_finish: st:gmac_state ->
+  s:tagB{disjoint st.r_acc s /\ disjoint st.pmsg s /\ disjoint st.len s} ->
+  tag:tagB{disjoint st.r_acc tag /\ disjoint st.pmsg tag /\ disjoint st.len tag /\ disjoint s tag} ->
+  Stack unit
+  (requires (fun h -> valid_st h st /\ live h s /\ live h tag))
+  (ensures (fun h0 _ h1 -> valid_st h0 st /\ live h0 s /\ live h0 tag /\ valid_st h1 st /\ live h1 s /\ live h1 tag /\
+    modifies_3 st.r_acc st.pmsg tag h0 h1 /\
+    reveal_sbytes (as_seq h1 tag) = gmac_finish_spec (as_pure_st h0 st) (as_seq h0 s)))
+let gmac_finish st s tag =
   let h0 = ST.get() in
-  let st_s = sub st.s_pmsg_len 0ul 16ul in
-  blit s 0ul st_s 0ul 16ul;
+  let acc = sub st.r_acc 1ul 1ul in
+  gmac_last_ st;
+  let sv = encodeB s in
+  let h' = ST.get() in
+  lemma_reveal_modifies_2 st.r_acc st.pmsg h0 h';
+  decodeB tag H128.(acc.(0ul) ^^ sv);
   let h1 = ST.get() in
-  (* valid_st h1 st *)
-  let st_len = sub st.s_pmsg_len 32ul 1ul in
-  assert(disjoint st_s st_len);
-  lemma_reveal_modifies_1 st_s h0 h1;
-  lemma_sub_spec st.s_pmsg_len 32ul 1ul h0;
-  lemma_sub_spec st.s_pmsg_len 32ul 1ul h1;
-  Seq.lemma_index_slice (as_seq h0 st.s_pmsg_len) 32 33 0;
-  Seq.lemma_index_slice (as_seq h1 st.s_pmsg_len) 32 33 0;
-  (* get_s h1 st = as_seq h0 s *)
-  Seq.lemma_eq_intro (Seq.slice (get_s h1 st) 0 16) (get_s h1 st);
-  Seq.lemma_eq_intro (Seq.slice (as_seq h0 s) 0 16) (as_seq h0 s);
-  Seq.lemma_eq_intro (get_s h1 st) (as_seq h0 s);
-  (* get_pmsg h1 st = get_pmsg h0 st *)
-  let st_pmsg = sub st.s_pmsg_len 16ul 16ul in
-  assert(disjoint st_s st_pmsg);
-  lemma_reveal_modifies_1 st_s h0 h1;
-  (* get_r h1 st = get_r h0 st *)
-  lemma_sub_spec st.r_acc 0ul 1ul h0;
-  lemma_sub_spec st.r_acc 0ul 1ul h1;
-  (* get_acc h1 st = get_acc h0 st *)
-  lemma_sub_spec st.r_acc 1ul 1ul h0;
-  lemma_sub_spec st.r_acc 1ul 1ul h1
+  lemma_reveal_modifies_1 tag h' h1;
+  lemma_intro_modifies_3 st.r_acc st.pmsg tag h0 h1
 
-inline_for_extraction private
-val gmac_init_acc: st:gmac_state -> Stack unit
-  (requires (fun h -> valid_st h st))
-  (ensures (fun h0 _ h1 -> valid_st h0 st /\ valid_st h1 st /\
-    modifies_1 st.r_acc h0 h1 /\
-    get_r h1 st = get_r h0 st /\ get_s h1 st = get_s h0 st /\
-    get_acc h1 st = zero /\ get_pmsg h1 st = get_pmsg h0 st))
-let gmac_init_acc st =
+abstract val gmac_onetimeauth: tag:tagB ->
+  msg:buffer H8.t{disjoint tag msg} ->
+  len:U32.t{U32.v len = length msg} ->
+  r:keyB{disjoint tag r /\ disjoint msg r} ->
+  s:tagB{disjoint tag s /\ disjoint msg s /\ disjoint r s} ->
+  Stack unit
+  (requires (fun h -> live h tag /\ live h msg /\ live h r /\ live h s))
+  (ensures (fun h0 _ h1 -> live h0 tag /\ live h0 msg /\ live h0 r /\ live h0 s /\
+    live h1 tag /\ live h1 msg /\ live h1 r /\ live h1 s /\
+    modifies_1 tag h0 h1 /\
+    reveal_sbytes (as_seq h1 tag) = gmac_spec (as_seq h0 msg) (as_seq h0 r) (as_seq h0 s)))
+let gmac_onetimeauth tag msg len r s =
   let h0 = ST.get() in
-  let st_acc = sub st.r_acc 1ul 1ul in
-  st_acc.(0ul) <- zero_128;
+  push_frame();
+  let h' = ST.get() in
+  let st = gmac_alloc() in
+  let h0' = ST.get() in
+  lemma_reveal_modifies_0 h' h0';
+  gmac_init st r;
+  let h1' = ST.get() in
+  lemma_reveal_modifies_2 st.r_acc st.len h0' h1';
+  gmac_update st msg len;
+  let h2' = ST.get() in
+  lemma_reveal_modifies_3 st.r_acc st.pmsg st.len h1' h2';
+  gmac_finish st s tag;
+  let h3' = ST.get() in
+  lemma_reveal_modifies_3 st.r_acc st.pmsg tag h2' h3';
+  pop_frame();
   let h1 = ST.get() in
-  (* get_r h1 st = get_r h0 st *)
-  let st_r = sub st.r_acc 0ul 1ul in
-  assert(disjoint st_acc st_r);
-  lemma_reveal_modifies_1 st_acc h0 h1;
-  (* get_acc h1 st = zero *)
-  fzero_lemma zero_128;
-  Seq.lemma_eq_intro (get_acc h1 st) zero;
-  (* get_s h1 st = get_s h0 st *)
-  lemma_sub_spec st.s_pmsg_len 0ul 16ul h0;
-  lemma_sub_spec st.s_pmsg_len 0ul 16ul h1;
-  (* get_pmsg h1 st = get_pmsg h0 st *)
-  lemma_sub_spec st.s_pmsg_len 16ul (h8_to_u32 (get h0 st.s_pmsg_len 32)) h0;
-  lemma_sub_spec st.s_pmsg_len 16ul (h8_to_u32 (get h1 st.s_pmsg_len 32)) h1
-
-inline_for_extraction private
-val gmac_init_pmsg: st:gmac_state -> Stack unit
-  (requires (fun h -> valid_st h st))
-  (ensures (fun h0 _ h1 -> valid_st h0 st /\ valid_st h1 st /\
-    modifies_1 st.s_pmsg_len h0 h1 /\
-    get_r h1 st = get_r h0 st /\ get_s h1 st = get_s h0 st /\
-    get_acc h1 st = get_acc h0 st /\ get_pmsg h1 st = Seq.createEmpty))
-let gmac_init_pmsg st =
-  let h0 = ST.get() in
-  let st_len = sub st.s_pmsg_len 32ul 1ul in
-  st_len.(0ul) <- uint8_to_sint8 0uy;
-  let h1 = ST.get() in
-  (* valid_st h1 st *)
-  lemma_sub_spec st.s_pmsg_len 32ul 1ul h1;
-  Seq.lemma_index_slice (as_seq h1 st.s_pmsg_len) 32 33 0;
-  (* get_s h1 st = get_s h0 st *)
-  let st_s = sub st.s_pmsg_len 0ul 16ul in
-  assert(disjoint st_len st_s);
-  lemma_reveal_modifies_1 st_len h0 h1;
-  (* get_pmsg h1 st = Seq.createEmpty *)
-  lemma_sub_spec st.s_pmsg_len 16ul (h8_to_u32 (get h1 st.s_pmsg_len 32)) h1;
-  Seq.lemma_eq_intro (get_pmsg h1 st) (Seq.createEmpty);
-  (* get_r h1 st = get_r h0 st *)
-  lemma_sub_spec st.r_acc 0ul 1ul h0;
-  lemma_sub_spec st.r_acc 0ul 1ul h1;
-  (* get_acc h1 st = get_acc h0 st *)
-  lemma_sub_spec st.r_acc 1ul 1ul h0;
-  lemma_sub_spec st.r_acc 1ul 1ul h1
-
-
-(* Main GMAC functions *)
-val gmac_init: st:gmac_state -> r:wordB_16{disjoint st.r_acc r /\ disjoint st.s_pmsg_len r} ->
-  s:tagB{disjoint st.r_acc s /\ disjoint st.s_pmsg_len s /\ disjoint r s} -> Stack unit
-  (requires (fun h -> valid_st h st /\ live h r /\ live h s))
-  (ensures (fun h0 _ h1 -> valid_st h0 st /\ live h0 r /\ live h0 s /\
-    valid_st h1 st /\ live h1 r /\ live h1 s /\ modifies_2 st.r_acc st.s_pmsg_len h0 h1 /\
-    as_pure_st h1 st == gmac_init_spec (as_seq h0 r) (as_seq h0 s)))
-let gmac_init st r s =
-  gmac_set_r st r;
-  gmac_set_s st s;
-  gmac_init_acc st;
-  gmac_init_pmsg st
-*)
+  lemma_intro_modifies_1 tag h0 h1
